Try 2 at refactoring, more successful.
Add sort declarations.

Fix automation breakage: swap vl and vl_ + updates for that

- Use vl_ instead of _vl.
So that Coq still defaults to `v` to name values.

theories/Dot/syn.v
@@ -3,91 +3,6 @@ From D.Dot Require Export dot_syn.
 (** After instantiating Autosubst, a few binding-related syntactic definitions
     that need not their own file. *)
 
-Definition to_subst (ρ: vls) : var → vl := foldr (λ v s, v .: s) ids ρ.
-
-Lemma to_subst_nil: to_subst [] = ids.
-Proof. trivial. Qed.
-
-Lemma to_subst_cons v ρ : to_subst (v :: ρ) = v .: to_subst ρ.
-Proof. trivial. Qed.
-Hint Rewrite to_subst_nil to_subst_cons : autosubst.
-
-Global Typeclasses Opaque to_subst.
-Global Opaque to_subst.
-
-Definition subst_sigma (σ: vls) (ρ: vls) := σ.|[to_subst ρ].
-
-Definition push_var (σ: vls) : vls := ids 0 :: σ.|[ren (+1)].
-Arguments push_var /.
-
-(** Create an identity environment of the given length. *)
-Fixpoint idsσ n: vls :=
-  match n with
-  | 0 => []
-  | S n => push_var (idsσ n)
-  end.
-
-(** When two substitutions are equivalent up to n. *)
-Definition eq_n_s (s1 s2: var → vl) n := ∀ x, x < n → s1 x = s2 x.
-Arguments eq_n_s /.
-
-(** [n]-closedness defines when some AST has at most [n] free variables (from [0] to [n - 1]). *)
-(** Here and elsewhere, we give one definition for values, using [subst], and
-    another for other ASTs, using [hsubst]. *)
-Definition nclosed_vl (v: vl) n :=
-  ∀ s1 s2, eq_n_s s1 s2 n → v.[s1] = v.[s2].
-
-Definition nclosed `{HSubst vl X} (t: X) n :=
-  ∀ s1 s2, eq_n_s s1 s2 n → t.|[s1] = t.|[s2].
-
-Definition nclosed_σ σ n := Forall (λ v, nclosed_vl v n) σ.
-Arguments nclosed_σ /.
-
-Notation cl_ρ ρ := (nclosed_σ ρ 0).
-
-(** The following ones are "direct" lemmas: deduce that an expression is closed
-    by knowing that its subexpression are closed. *)
-
-(** Needed by solve_fv_congruence when dealing with binders, such as in fv_vobj and fv_vabs. *)
-Lemma eq_up s1 s2 n: eq_n_s s1 s2 n → eq_n_s (up s1) (up s2) (S n).
-Proof.
-  rewrite /up. move => Heq [|x] Hl //=. f_equiv. apply Heq. lia.
-Qed.
-
-(** Automated proof for such lemmas. *)
-Ltac solve_fv_congruence :=
-  rewrite /nclosed /nclosed_vl => * /=; repeat (f_equiv; try solve [(idtac + asimpl); auto using eq_up]).
-
-Lemma fv_cons `{Ids X} `{HSubst vl X} {hsla: HSubstLemmas vl X} (x: X) xs n: nclosed xs n → nclosed x n → nclosed (x :: xs) n.
-Proof. solve_fv_congruence. Qed.
-
-Lemma fv_pair_cons {A} `{Ids X} `{HSubst vl X} {hsla: HSubstLemmas vl X} (a: A) (x: X) xs n: nclosed xs n → nclosed x n → nclosed ((a, x) :: xs) n.
-Proof. solve_fv_congruence. Qed.
-
-(** The following ones are "inverse" lemmas: by knowing that an expression is closed,
-    deduce that one of its subexpressions is closed *)
-
-(** Dealing with binders in fv "inverse" lemmas requires more infrastructure. See fv_vabs_inv_manual for an explanation. *)
-
-Definition stail s := ren (+1) >> s.
-Definition shead (s: var → vl) := s 0.
-
-Lemma eq_n_s_tails {n s1 s2}: eq_n_s s1 s2 (S n) → eq_n_s (stail s1) (stail s2) n.
-Proof. rewrite /stail => /= HsEq x Hl. apply HsEq. lia. Qed.
-Lemma eq_n_s_heads {n s1 s2}: eq_n_s s1 s2 n → n > 0 → shead s1 = shead s2.
-Proof. rewrite /shead => /= HsEq. apply HsEq. Qed.
-
-Lemma decomp_s `{Ids A} `{HSubst vl A} {hsla: HSubstLemmas vl A} (a: A) s:
-  a.|[s] = a.|[up (stail s)].|[shead s/].
-Proof. by rewrite /stail /shead; asimpl. Qed.
-
-Lemma decomp_s_vl v s:
-  v.[s] = v.[up (stail s)].[shead s/].
-Proof. by rewrite /stail /shead; asimpl. Qed.
-
-(** Rewrite thesis with equalities learned from injection, if possible *)
-Ltac rewritePremises := let H := fresh "H" in repeat (move => H; rewrite ?H {H}).
-
 (** Here is a manual proof of a lemma, with explanations. *)
 Lemma fv_vabs_inv_manual e n: nclosed_vl (vabs e) n → nclosed e (S n).
 Proof.
@@ -102,35 +17,6 @@ Proof.
   rewrite ?(decomp_s _ s1) ?(decomp_s _ s2) ?(decomp_s_vl _ s1) ?(decomp_s_vl _ s2) (eq_n_s_heads HsEq); last lia.
   injection (Hfv _ _ (eq_n_s_tails HsEq)); rewritePremises; reflexivity.
 Qed.
-
-(** Finally, a heuristic solver [solve_inv_fv_congruence] to be able to prove
-    such lemmas easily, both here and elsewhere. *)
-
-Ltac solve_inv_fv_congruence :=
-  let s1 := fresh "s1" in
-  let s2 := fresh "s2" in
-  let HsEq := fresh "HsEq" in
-  let Hfv := fresh "Hfv" in
-  rewrite /nclosed_vl /nclosed /= => Hfv s1 s2 HsEq;
-(* asimpl is expensive, but sometimes needed when simplification does mistakes.
-   It must also be done after injection because it might not rewrite under Hfv's
-   binders. *)
-  by [ injection (Hfv s1 s2); trivial; by (idtac + asimpl; rewritePremises; reflexivity) |
-       rewrite ?(decomp_s _ s1) ?(decomp_s _ s2) ?(decomp_s_vl _ s1) ?(decomp_s_vl _ s2) (eq_n_s_heads HsEq); last lia;
-       injection (Hfv _ _ (eq_n_s_tails HsEq)); by rewritePremises ].
-
-Ltac solve_inv_fv_congruence_h Hcl :=
-  move: Hcl; solve_inv_fv_congruence.
-
-Ltac solve_inv_fv_congruence_auto :=
-  match goal with
-  | Hcl: nclosed ?t ?n |- nclosed _ _ => solve_inv_fv_congruence_h Hcl
-  | Hcl: nclosed_vl ?t ?n |- nclosed _ _ => solve_inv_fv_congruence_h Hcl
-  | Hcl: nclosed ?t ?n |- nclosed_vl _ _ => solve_inv_fv_congruence_h Hcl
-  | Hcl: nclosed_vl ?t ?n |- nclosed_vl _ _ => solve_inv_fv_congruence_h Hcl
-  end.
-
-Hint Extern 10 => solve_inv_fv_congruence_auto: fv.
 
 (* Special cases needed below. *)
 
