theories/asubst_lemmas.v
@@ -1,0 +1,359 @@
+From D Require Import prelude tactics asubst_base.
+
+Module SortsLemmas (values: Values).
+  Import values.
+  Module M := Sorts values.
+  Import M.
+  (* TODO Next: provide instances, and move synLemmas in here. *)
+  Section sort_lemmas.
+    Context `{Sort X}.
+
+  Lemma length_idsσr n r: length (idsσ n).|[ren r] = n.
+  Proof.
+    elim : n r => [r | n IHn r] => //.
+    asimpl. by rewrite IHn.
+  Qed.
+
+  Lemma length_idsσ n: length (idsσ n) = n.
+  Proof. pose proof (length_idsσr n (+0)) as Hr. asimpl in Hr. exact Hr. Qed.
+  Hint Resolve length_idsσ.
+
+  Lemma subst_sigma_idsσ ρ n : length ρ = n →
+                  (subst_sigma (idsσ n) ρ) = ρ.
+  Proof.
+    rewrite /subst_sigma. move :n.
+    induction ρ => *; subst => //; asimpl.
+    f_equal. by apply IHρ.
+  Qed.
+
+  Lemma to_subst_app_is_lookup ρ x: x < length ρ → ρ !! x = Some (to_subst ρ x).
+  Proof.
+    elim :ρ x => [|v ρ IHρ] [|x] //= Hl; try lia.
+    rewrite to_subst_cons /=.
+    apply IHρ; lia.
+  Qed.
+
+  Lemma rename_to_subst ρ1 ρ2 : (+length ρ1) >>> to_subst (ρ1 ++ ρ2) = to_subst ρ2.
+  Proof. induction ρ1; by asimpl. Qed.
+
+  Lemma undo_to_subst ρ : (+length ρ) >>> to_subst ρ = ids.
+  Proof.
+    pose proof (rename_to_subst ρ []) as Hr. rewrite app_nil_r in Hr. asimpl in Hr. exact Hr.
+  Qed.
+
+  Lemma to_subst_weaken ρ1 ρ2 ρ3:
+    upn (length ρ1) (ren (+length ρ2)) >> to_subst (ρ1 ++ ρ2 ++ ρ3) =
+    to_subst (ρ1 ++ ρ3).
+  Proof.
+    induction ρ1; asimpl.
+    - by rewrite rename_to_subst.
+    - by f_equal.
+  Qed.
+
+  Lemma to_subst_up ρ1 ρ2 v:
+    upn (length ρ1) (v.[ren (+length ρ2)] .: ids) >> to_subst (ρ1 ++ ρ2) =
+    to_subst (ρ1 ++ v :: ρ2).
+  Proof.
+    induction ρ1; asimpl.
+    - rewrite undo_to_subst. by asimpl.
+    - by f_equal.
+  Qed.
+
+  Lemma closed_subst_vl_id v σ: nclosed_vl v 0 → v.[σ] = v.
+  Proof.
+    intro Hcl. rewrite (Hcl σ ids) /=; first by asimpl.
+    intros; lia.
+  Qed.
+  (* Implicit Type (x: X). *)
+
+  Lemma closed_subst_id (x: X) σ: nclosed x 0 → x.|[σ] = x.
+  Proof.
+    intro Hcl. rewrite (Hcl σ ids) /=; first by asimpl.
+    intros; lia.
+  Qed.
+
+  Lemma closed_to_subst ρ i n: nclosed_σ ρ n → i < length ρ → nclosed_vl (to_subst ρ i) n.
+  Proof.
+    elim: ρ i => /= [|v ρ IHρ] [|i] Hcl Hl; asimpl; try lia; inverse Hcl; try by [].
+    by apply IHρ; try lia.
+  Qed.
+
+  (** Let's prove that [nclosed a n → a.|[to_subst (idsσ n)] = a], and ditto for values. *)
+  Section to_subst_idsσ_is_id.
+    Lemma to_subst_map_commute_aux f n x r: x < n → to_subst (map f (idsσ n).|[ren r]) x = f (to_subst (idsσ n).|[ren r] x).
+    Proof.
+      elim: n r x => [|n IHn] r x Hle; first lia.
+      destruct x; first done; asimpl.
+      apply IHn; lia.
+    Qed.
+
+    Lemma to_subst_map_commute f n x: x < n → to_subst (map f (idsσ n)) x = f (to_subst (idsσ n) x).
+    Proof. pose proof (to_subst_map_commute_aux f n x (+0)) as Hr. asimpl in Hr. exact Hr. Qed.
+
+    Lemma idsσ_eq_ids n: eq_n_s (to_subst (idsσ n)) ids n.
+    Proof.
+      induction n => x Hle. by rewrite to_subst_nil.
+      destruct x => //=.
+      assert (x < n) as Hle' by auto using lt_S_n.
+      by rewrite to_subst_cons /= to_subst_map_commute // IHn // id_subst.
+    Qed.
+
+    Lemma closed_subst_idsρ (x:X) n :
+      nclosed x n → x.|[to_subst (idsσ n)] = x.
+    Proof.
+      intro Hcl. rewrite (Hcl _ ids); first by asimpl. by apply idsσ_eq_ids.
+    Qed.
+
+    Lemma closed_subst_vl_idsρ v n:
+      nclosed_vl v n → v.[to_subst (idsσ n)] = v.
+    Proof.
+      intro Hcl. rewrite (Hcl _ ids); first by asimpl. by apply idsσ_eq_ids.
+    Qed.
+  End to_subst_idsσ_is_id.
+
+  Lemma fv_to_subst (x: X) σ n:
+    nclosed x (length σ) → nclosed_σ σ n →
+    nclosed (x.|[to_subst σ]) n.
+  Proof.
+    rewrite /nclosed /nclosed_vl => Hcla Hclρ s1 s2 Heqsn /=; asimpl.
+    apply Hcla.
+    intros i Hl; asimpl. by eapply (closed_to_subst σ i n).
+  Qed.
+
+  Lemma fv_to_subst_vl v σ n:
+    nclosed_vl v (length σ) → nclosed_σ σ n →
+    nclosed_vl (v.[to_subst σ]) n.
+  Proof.
+    rewrite /nclosed /nclosed_vl => Hclv Hclσ s1 s2 Heqsn /=; asimpl.
+    apply Hclv.
+    intros x Hl; asimpl. by eapply (closed_to_subst σ x n).
+  Qed.
+
+  (** Variants of [fv_to_subst] and [fv_to_subst_vl] for more convenient application. *)
+  Lemma fv_to_subst' (x:X) σ x' n:
+    nclosed x (length σ) → nclosed_σ σ n →
+    x' = (x.|[to_subst σ]) →
+    nclosed x' n.
+  Proof. intros; subst. by apply fv_to_subst. Qed.
+  Lemma fv_to_subst_vl' v σ v' n:
+    nclosed_vl v (length σ) → nclosed_σ σ n →
+    v' = (v.[to_subst σ]) →
+    nclosed_vl v' n.
+  Proof. intros; subst. by apply fv_to_subst_vl. Qed.
+
+  Implicit Types
+          (Γ : list X) (ρ : vls).
+
+  Lemma lookup_var Γ x T: Γ !! x = Some T → nclosed_vl (ids x) (length Γ).
+  Proof. rewrite /nclosed /nclosed_vl => *; rewrite !id_subst. eauto using lookup_lt_Some. Qed.
+
+  Lemma nclosed_var_lt i n: nclosed_vl (ids i) n -> i < n.
+  Proof.
+    rewrite /nclosed_vl /= => Heq.
+    set s0 := fun k x => (if (decide (x < n)) then ids 0 else ids k): vl.
+    set s1 := s0 1; set s2 := s0 2. subst s0.
+    have Heqs: eq_n_s s1 s2 n. by subst s1 s2; move=> ??; case_decide.
+    specialize (Heq s1 s2 Heqs); move: Heq {Heqs}; subst s1 s2 => /=.
+    rewrite !id_subst. by case_decide => // /inj_ids.
+  Qed.
+
+  Lemma nclosed_vl_ids_0 i: i > 0 → nclosed_vl (ids 0) i.
+  Proof. move => Hi s1 s2 /= Heqs. rewrite !id_subst. by apply Heqs. Qed.
+
+  Lemma nclosed_vl_ids_S i j: nclosed_vl (ids i) j → nclosed_vl (ids (S i)) (S j).
+  Proof.
+    move => /= Hij s1 s2 Heqs. rewrite !id_subst. apply: Heqs.
+    suff: i < j by lia. by apply nclosed_var_lt.
+  Qed.
+
+  Lemma nclosed_vl_ids i j: i < j → nclosed_vl (ids i) j.
+  Proof. move => ????; rewrite !id_subst. eauto. Qed.
+
+  Hint Resolve nclosed_var_lt nclosed_vl_ids_0 nclosed_vl_ids_S nclosed_vl_ids.
+
+  Lemma nclosed_vl_ids_equiv i j: nclosed_vl (ids i) j <-> i < j.
+  Proof. split; eauto. Qed.
+
+  Lemma nclosed_ids_rev i j x:
+    nclosed_vl (ids x).[ren (+j)] (j + i) → nclosed_vl (ids x) i.
+  Proof. asimpl. rewrite !nclosed_vl_ids_equiv. lia. Qed.
+
+  (** Not yet used. *)
+  Lemma eq_n_s_mon n m {s1 s2}: eq_n_s s1 s2 m → n < m → eq_n_s s1 s2 n.
+  Proof. rewrite /eq_n_s => HsEq Hnm x Hl. apply HsEq; lia. Qed.
+
+  Lemma nclosed_mono (x:X) n m: nclosed x n → n < m → nclosed x m.
+  Proof. move => Hcl Hle s1 s2 Hseq. by eapply Hcl, eq_n_s_mon. Qed.
+
+  (* Definition fv_dms_cons : ∀ l d ds n, nclosed ds n → nclosed d n → nclosed ((l, d) :: ds) n := fv_pair_cons. *)
+
+  Lemma fv_vls_cons (v:vl) (vs:vls) n: nclosed vs n → nclosed_vl v n → nclosed (v :: vs) n.
+  Proof. solve_fv_congruence. Qed.
+
+  Lemma nclosed_ids x n: nclosed_vl (ids x) (S (x + n)).
+  Proof. move => /= s1 s2 Heq. rewrite !id_subst. apply Heq. lia. Qed.
+
+  Lemma nclosed_idsσr n x: nclosed_σ (idsσ n).|[ren (+x)] (x + n).
+  Proof.
+    elim: n x => [|n IHn] x //=.
+    constructor; asimpl; [apply nclosed_ids | apply (IHn (S x)) ].
+  Qed.
+
+  Lemma nclosed_idsσ n: nclosed_σ (idsσ n) n.
+  Proof. pose proof nclosed_idsσr n 0 as Hr; asimpl in Hr; exact Hr. Qed.
+  Hint Resolve nclosed_idsσ.
+
+  (* Definition nclosed_ds ds n := Forall (λ '(l, d), nclosed d n) ds. *)
+  (* Global Arguments nclosed_ds /. *)
+
+  (* Lemma Forall_to_closed_dms n ds: *)
+  (*   nclosed_ds ds n → nclosed ds n. *)
+  (* Proof. *)
+  (*   elim: ds => [|[l d] ds IHds] Hcl //=. *)
+  (*   inverse Hcl; apply fv_dms_cons; by [ apply IHds | ]. *)
+  (* Qed. *)
+  (* Lemma closed_dms_to_Forall n ds: *)
+  (*   nclosed ds n → nclosed_ds ds n. *)
+  (* Proof. *)
+  (*   elim: ds => [|[l d] ds IHds] Hcl //=. *)
+  (*   constructor. solve_inv_fv_congruence_h Hcl. *)
+  (*   apply IHds. solve_inv_fv_congruence_h Hcl. *)
+  (* Qed. *)
+
+  Lemma Forall_to_closed_vls n σ:
+    nclosed_σ σ n → nclosed σ n.
+  Proof.
+    elim: σ => [|v σ IHσ] Hcl //=.
+    inverse Hcl; apply fv_vls_cons; by [ apply IHσ | ].
+  Qed.
+
+  Lemma closed_vls_to_Forall m σ:
+    nclosed σ m -> nclosed_σ σ m.
+  Proof.
+    elim: σ => [|v σ IHσ] Hcl //=.
+    constructor. solve_inv_fv_congruence_h Hcl.
+    apply IHσ. solve_inv_fv_congruence_h Hcl.
+  Qed.
+
+  Definition cl_ρ_fv: ∀ ρ, cl_ρ ρ → nclosed ρ 0 := Forall_to_closed_vls 0.
+
+  Lemma fv_idsσ n: nclosed (idsσ n) n.
+  Proof. apply Forall_to_closed_vls, nclosed_idsσ. Qed.
+
+  Lemma fv_idsσ_alt n: nclosed (idsσ n) n.
+  Proof.
+    rewrite /nclosed. elim: n => [|n] //= IHn s1 s2 Heq. asimpl.
+    f_equiv; [| apply IHn; intros]; apply Heq => /=; lia.
+  Qed.
+
+  Lemma to_subst_compose σ σ':
+    eq_n_s (to_subst σ.|[σ']) (to_subst σ >> σ') (length σ).
+  Proof.
+    induction σ as [| v σ] => /= x Hxn; first lia; asimpl.
+    destruct x => //=.
+    (* elim: σ => /= [|v σ IHσ] x Hxn; first lia; asimpl. *)
+    (* case: x Hxn => [|x] Hxn //=. *)
+    apply IHσ. lia.
+  Qed.
+
+  Lemma to_subst_compose_alt σ σ' n:
+    n = length σ →
+    eq_n_s (to_subst σ.|[σ']) (to_subst σ >> σ') n.
+  Proof. intros; subst. apply to_subst_compose. Qed.
+
+  Lemma subst_compose_x (x: X) σ ξ n1 n2 n3:
+    nclosed x n1 →
+    length σ = n1 → nclosed_σ σ n2 →
+    length ξ = n2 → nclosed_σ ξ n3 →
+    x.|[to_subst σ.|[to_subst ξ]] = x.|[to_subst σ].|[to_subst ξ].
+  Proof.
+    intros HclA Hlenσ Hclσ Hlenξ Hclξ.
+    asimpl. apply HclA. subst. by apply to_subst_compose.
+  Qed.
+  Hint Resolve subst_compose_x.
+
+  Lemma subst_compose_idsσ_x (x:X) n m ξ:
+    nclosed x n →
+    nclosed_σ ξ m →
+    length ξ = n →
+    x.|[to_subst (idsσ n).|[to_subst ξ]] = x.|[to_subst (idsσ n)].|[to_subst ξ].
+  Proof. intros; eauto. Qed.
+
+  End sort_lemmas.
+  Hint Resolve nclosed_var_lt nclosed_vl_ids_0 nclosed_vl_ids_S nclosed_vl_ids.
+  Hint Resolve nclosed_idsσ @subst_compose_x @subst_compose_idsσ_x.
+
+  Section sort_lemmas_2.
+    Context `{Sort X}.
+    Implicit Types (x: X).
+
+    Lemma nclosed_σ_to_subst ξ σ n:
+      nclosed_σ ξ (length σ) → nclosed_σ σ n →
+      nclosed_σ (ξ.|[to_subst σ]) n.
+    Proof.
+      intros.
+      apply closed_vls_to_Forall, fv_to_subst => //. by apply Forall_to_closed_vls.
+    Qed.
+
+    Definition nclosed_sub n m s :=
+      ∀ i, i < n → nclosed_vl (s i) m.
+    Definition nclosed_ren n m (r: var → var) := nclosed_sub n m (ren r).
+
+    Lemma compose_sub_closed s s1 s2 i j:
+      nclosed_sub i j s → eq_n_s s1 s2 j → eq_n_s (s >> s1) (s >> s2) i.
+    Proof. move => /= Hs Heqs x Hxi. exact: Hs. Qed.
+
+    Lemma nclosed_ren_shift n m j:
+      m >= j + n → nclosed_ren n m (+j).
+    Proof. move=>???/=; eauto with lia. Qed.
+    Hint Resolve nclosed_ren_shift.
+
+    Lemma nclosed_sub_vl v s i j:
+      nclosed_sub i j s →
+      nclosed_vl v i → nclosed_vl v.[s] j.
+    Proof. move => Hcls Hclv s1 s2 Heqs; asimpl. by eapply Hclv, compose_sub_closed. Qed.
+
+    Lemma nclosed_sub_x (x: X) s i j:
+      nclosed_sub i j s →
+      nclosed x i → nclosed x.|[s] j.
+    Proof. move => Hcls Hcla s1 s2 Heqs; asimpl. by eapply Hcla, compose_sub_closed. Qed.
+
+    Lemma nclosed_ren_vl v r i j:
+      nclosed_ren i j r →
+      nclosed_vl v i → nclosed_vl (rename r v) j.
+    Proof. (* asimpl. *)
+      rewrite rename_subst. exact: nclosed_sub_vl.
+    Qed.
+
+    Lemma nclosed_sub_up i j s:
+      nclosed_sub i j s →
+      nclosed_sub (S i) (S j) (up s).
+    Proof.
+      move => //= Hs [|x] Hx; asimpl. eauto with lia.
+      asimpl; rewrite -rename_subst.
+      eapply nclosed_ren_vl; by eauto with lia.
+    Qed.
+    Hint Resolve nclosed_sub_up.
+
+    Lemma nclosed_ren_up n m r:
+      nclosed_ren n m r →
+      nclosed_ren (S n) (S m) (upren r).
+    Proof. move => //= Hr [|i] Hi; asimpl; eauto with lia. Qed.
+    Hint Resolve nclosed_ren_up.
+
+    Lemma nclosed_sub_inv_var n w i j k: j + k <= i →
+      nclosed_vl (ids n).[upn j (w .: ids) >> ren (+k)] i →
+      nclosed_vl (ids n) (S i).
+    Proof.
+      rewrite !id_subst /= !nclosed_vl_ids_equiv iter_up.
+      case: (lt_dec n j) => [?|Hge]; first lia.
+      case Hnj: (n - j) => [|nj]; first lia.
+      rewrite rename_subst !id_subst.
+      rewrite nclosed_vl_ids_equiv /=. lia.
+    Qed.
+
+  End sort_lemmas_2.
+
+  Hint Resolve nclosed_σ_to_subst.
+
+End SortsLemmas.
